WIP using autosubst

theories/syntax_systemF.v
@@ -1,45 +1,55 @@
 Set Warnings "-notation-overridden,-parsing,-deprecated-hint-without-locality".
 From Coq Require Import Strings.String.
 From stdpp Require Import gmap list.
+Require Import Autosubst.Autosubst.
 From logical_relation Require Import relation.
 
 Inductive ty : Type :=
-| Ty_Var : string -> ty
+| Ty_Var : var -> ty
 | Ty_Unit : ty
 | Ty_Pair : ty -> ty -> ty
 | Ty_Arrow : ty -> ty -> ty
-| Ty_Forall : string -> ty -> ty.
+| Ty_Forall : {bind ty} -> ty.
+
+Instance Ids_ty : Ids ty. derive. Defined.
+Instance Rename_ty : Rename ty. derive. Defined.
+Instance Subst_ty : Subst ty. derive. Defined.
+Instance SubstLemmas_ty : SubstLemmas ty. derive. Qed.
 
 Inductive expr : Type :=
-| expr_var : string -> expr
+| expr_var : var -> expr
 | expr_unit : expr
 | expr_pair : expr -> expr -> expr
 | expr_fst : expr -> expr
 | expr_snd : expr -> expr
 | expr_app : expr -> expr -> expr
-| expr_abs : string -> expr -> expr
+| expr_lam : {bind expr} -> expr
 | expr_tapp : expr -> expr
-| expr_tabs : expr -> expr.
+| expr_tlam : expr -> expr.
 Inductive val :=
 | val_unit : val
 | val_pair : val -> val -> val
-| val_abs : string -> expr -> val
-| val_tabs : expr -> val
-.
+| val_lam : {bind expr} -> val
+| val_tlam : expr -> val.
+
+Instance Ids_expr : Ids expr. derive. Defined.
+Instance Rename_expr : Rename expr. derive. Defined.
+Instance Subst_expr : Subst expr. derive. Defined.
+Instance SubstLemmas_expr : SubstLemmas expr. derive. Qed.
 
 Fixpoint of_val (v : val) : expr :=
   match v with
   | val_unit => expr_unit
   | val_pair v1 v2 => expr_pair (of_val v1) (of_val v2)
-  | val_abs s e => expr_abs s e
-  | val_tabs e => expr_tabs e
+  | val_lam e => expr_lam e
+  | val_tlam e => expr_tlam e
   end.
 
 Fixpoint to_val (e : expr) : option val :=
   match e with
   | expr_unit => Some val_unit
-  | expr_abs s e => Some (val_abs s e)
-  | expr_tabs e => Some (val_tabs e)
+  | expr_lam e => Some (val_lam e)
+  | expr_tlam e => Some (val_tlam e)
   | expr_pair e1 e2 =>
       match (to_val e1) with
       | None => None
@@ -54,12 +64,11 @@ Fixpoint to_val (e : expr) : option val :=
 
 Inductive is_val : expr -> Prop :=
 | v_unit : is_val expr_unit
-| v_pair : forall v1 v2, is_val v1 -> is_val v2 -> is_val (expr_pair v1 v2)
-| v_abs : forall x t1, is_val (expr_abs x t1)
-| v_tabs : forall t1, is_val (expr_tabs t1).
+| v_pair : forall e1 e2, is_val e1 -> is_val e2 -> is_val (expr_pair e1 e2)
+| v_lam : forall e, is_val (expr_lam e)
+| v_tlam : forall e, is_val (expr_tlam e).
 
 Hint Constructors is_val : core.
-
 
 (** Equality  *)
 Lemma to_of_val v : to_val (of_val v) = Some v.
@@ -67,9 +76,9 @@ Proof.
   by induction v; simplify_option_eq; repeat f_equal; try apply (proof_irrel _).
 Qed.
 
-Lemma of_to_val e v : to_val e = Some v → of_val v = e.
+Lemma of_to_val e ev : to_val e = Some ev → of_val ev = e.
 Proof.
-  revert v; induction e; intros v ?; simplify_option_eq; auto with f_equal.
+  revert ev; induction e; intros ev ?; simplify_option_eq; auto with f_equal.
   destruct (to_val e1); simpl;[|  discriminate].
   destruct (to_val e2); simpl;[|  discriminate].
   simplify_option_eq; auto with f_equal.
@@ -81,8 +90,8 @@ Proof.
   induction v; simpl.
   apply v_unit.
   apply v_pair; done.
-  apply v_abs.
-  apply v_tabs.
+  apply v_lam.
+  apply v_tlam.
 Qed.
 
 
@@ -92,8 +101,8 @@ Notation "x" := x (in custom sf at level 0, x constr at level 0).
 Notation "S -> T" := (Ty_Arrow S T) (in custom sf at level 50, right associativity).
 Notation "S × T" := (Ty_Pair S T) (in custom sf at level 50, right associativity).
 Notation "'()'" := Ty_Unit (in custom sf at level 0).
-Notation "∀ α , T" := (Ty_Forall α T) (in custom sf at level 50).
-Coercion expr_var : string >-> expr.
+Notation "∀ '_' , T" := (Ty_Forall T) (in custom sf at level 50).
+Coercion expr_var : var >-> expr.
 Notation "'tt'" := expr_unit (in custom sf at level 0).
 Notation "'⟨' e1 ',' e2 '⟩'" := (expr_pair e1 e2) (in custom sf at level 90,
                                       e1 at level 99,
@@ -101,151 +110,55 @@ Notation "'⟨' e1 ',' e2 '⟩'" := (expr_pair e1 e2) (in custom sf at level 90,
 Notation "'fst' e" := (expr_fst e) (in custom sf at level 2).
 Notation "'snd' e" := (expr_snd e) (in custom sf at level 2).
 Notation "e1 e2" := (expr_app e1 e2) (in custom sf at level 1, left associativity).
-Notation "'λ' x ',' y" :=
-  (expr_abs x y) (in custom sf at level 90, x at level 99,
+Notation "'λ' '_' ',' y" :=
+  (expr_lam y) (in custom sf at level 90,
         y custom sf at level 99,
         left associativity).
 Notation "e1 '_'" := (expr_tapp e1) (in custom sf at level 1, left associativity).
 Notation "'Λ' e" :=
-  (expr_tabs e) (in custom sf at level 90,
+  (expr_tlam e) (in custom sf at level 90,
         e custom sf at level 99,
         left associativity).
 
-Definition x : string := "x".
-Definition y : string := "y".
-Definition z : string := "z".
-Definition α : string := "α".
-Hint Unfold x : core.
-Hint Unfold y : core.
-Hint Unfold z : core.
-Hint Unfold α : core.
-
-Fixpoint subst_term (x : string) (s : expr) (t : expr) : expr :=
-  match t with
-  | expr_var y =>
-      if String.eqb x y then s else t
-  | <{ tt }> =>  <{ tt }>
-  | <{ ⟨t1, t2⟩ }> =>
-      <{ ⟨ (subst_term x s t1) , (subst_term x s t2) ⟩ }>
-  | <{fst t1}> => <{fst (subst_term x s t1)}>
-  | <{snd t1}> => <{snd (subst_term x s t1)}>
-  | <{ t1 t2 }> =>
-      <{ (subst_term x s t1) (subst_term x s t2) }>
-  | <{ λ y, t1 }> =>
-      if String.eqb x y then t else <{ λ y, (subst_term x s t1) }>
-  | <{ t1 _ }> => <{ (subst_term x s t1) _ }>
-  | <{ Λ t1 }> => <{ Λ (subst_term x s t1) }>
-  end.
-
-Notation "'[' x '/' s ']' t" := (subst_term x s t) (in custom sf at level 20).
-
-Fixpoint subst_type (α : string) (s : ty) (t : ty) : ty :=
-  match t with
-  | Ty_Var β => if String.eqb α β then s else t
-  | Ty_Unit => Ty_Unit
-  | <{ τ1 × τ2 }> => <{ (subst_type α s τ1) × (subst_type α s τ2) }>
-  | <{ τ1 -> τ2 }> => <{ (subst_type α s τ1) -> (subst_type α s τ2) }>
-  | <{ ∀ β , τ1  }> => if String.eqb α β then t else <{ ∀ β , (subst_type α s τ1) }>
-  end.
-Notation "'[' α ':=' s ']' t" := (subst_type α s t) (in custom sf at level 20).
-
-(* TODO simultaneous substitution ?? better way ?*)
-Fixpoint replace_var xs vs y t : expr :=
-  match xs,vs with
-  | nil, _ => t
-  | x::xs', nil => t
-  | x::xs', v::vs' =>
-      if String.eqb x y
-      then v
-      else replace_var xs' vs' y t
-  end.
-
-Fixpoint subst_term_seq (xs : list string) (vs : list expr) (t : expr) : expr :=
-  match t with
-  | expr_var y => replace_var xs vs y t
-  | <{ tt }> =>  <{ tt }>
-  | <{ ⟨t1, t2⟩ }> =>
-      <{ ⟨ (subst_term_seq xs vs t1) , (subst_term_seq xs vs t2) ⟩ }>
-  | <{fst t1}> => <{fst (subst_term_seq xs vs t1)}>
-  | <{snd t1}> => <{snd (subst_term_seq xs vs t1)}>
-  | <{ t1 t2 }> =>
-      <{ (subst_term_seq xs vs t1) (subst_term_seq xs vs t2) }>
-  | <{ λ y, t1 }> =>
-      match List.find (String.eqb y) xs with
-      | None => <{ λ y, (subst_term_seq xs vs t1) }>
-      | Some x => t
-      end
-  | <{ t1 _ }> => <{ (subst_term_seq xs vs t1) _ }>
-  | <{ Λ t1 }> => <{ Λ (subst_term_seq xs vs t1) }>
-  end.
 
 (* Use gmap ? My own partial map ? list ? *)
-Definition context := gmap string ty.
-Definition tcontext := gset string.
+Definition context := gmap var ty.
+(* Definition tcontext := gset var. *)
 
 (* TODO notation / definition for the empty context and tcontext *)
 
-Reserved Notation "Δ ';' Γ '⊢' t '∈' T"
+Reserved Notation "Δ '⊢' t '∈' T"
   (at level 101, t custom sf, T custom sf at level 0).
 
-Inductive appears_free_in (x : string) : expr → Prop :=
-| afi_var : appears_free_in x <{x}>
-| afi_pair1 : ∀ t1 t2,
-  appears_free_in x t1 →
-  appears_free_in x <{ ⟨t1, t2⟩ }>
-| afi_pair2 : ∀ t1 t2,
-  appears_free_in x t2 →
-  appears_free_in x <{ ⟨t1, t2⟩ }>
-| afi_app1 : ∀ t1 t2,
-  appears_free_in x t1 →
-  appears_free_in x <{t1 t2}>
-| afi_app2 : ∀ t1 t2,
-  appears_free_in x t2 →
-  appears_free_in x <{t1 t2}>
-| afi_abs : ∀ y t1,
-  y ≠ x →
-  appears_free_in x t1 →
-  appears_free_in x <{ λ y, t1}>.
-
-Inductive free (α : string) : ty -> Prop :=
-| free_var : free α (Ty_Var α)
-| free_pair1 : forall τ1 τ2, free α τ1 -> free α <{ τ1 × τ2 }>
-| free_pair2 : forall τ1 τ2, free α τ2 -> free α <{ τ1 × τ2 }>
-| free_arrow1 : forall τ1 τ2, free α τ1 -> free α <{ τ1 -> τ2 }>
-| free_arrow2 : forall τ1 τ2, free α τ2  -> free α <{ τ1 -> τ2 }>
-| free_forall : forall τ β, α ≠ β -> free α τ -> free α <{ ∀ β, τ }>.
-
-Definition not_free_context (α : string) (Γ : context) :=
-forall x y, Γ !! x = Some y -> not (free α y).
-
-Inductive typing_judgment : tcontext -> context -> expr -> ty -> Prop :=
-| T_Unit: forall Δ Γ, Δ;Γ ⊢ tt ∈ ()
-| T_Var: forall Δ Γ τ (x : string), Γ !! x = Some τ -> Δ;Γ ⊢ x ∈ τ
-| T_Prod: forall Δ Γ e1 τ1 e2 τ2,
-  Δ;Γ ⊢ e1 ∈ τ1 ->
-    Δ;Γ ⊢ e2 ∈ τ2 ->
-      Δ;Γ ⊢ ⟨e1, e2⟩ ∈ <{ τ1 × τ2 }>
-| T_Fst: forall Δ Γ e τ1 τ2,
-  Δ;Γ ⊢ e ∈ <{ τ1 × τ2 }> ->
-    Δ;Γ ⊢ fst e ∈ τ1
-| T_Snd: forall Δ Γ e τ1 τ2,
-  Δ;Γ ⊢ e ∈ <{ τ1 × τ2 }> ->
-    Δ;Γ ⊢ snd e ∈ τ2
-| T_Lam: forall Δ Γ x e τ1 τ2,
-  Δ;(<[x:=τ1]> Γ) ⊢ e ∈ τ2 ->
-    Δ;Γ ⊢ <{ λ x , e }> ∈ <{ τ1 -> τ2 }>
-| T_App: forall Δ Γ e e' τ1 τ2,
-  Δ;Γ ⊢ e ∈ <{ τ1 -> τ2 }> ->
-    Δ;Γ ⊢ e' ∈ τ1 ->
-      Δ;Γ ⊢ e e' ∈ τ2
-| T_TLam: forall Δ Γ e α τ,
-  ({[α]} ∪ Δ);Γ ⊢ e ∈ τ ->
-          not_free_context α Γ ->
-          Δ;Γ ⊢ Λ e ∈ <{ ∀ α , τ }>
-| T_TApp: forall Δ Γ e α τ τ',
-  Δ;Γ ⊢ e ∈ <{ ∀ α , τ }> ->
-    Δ;Γ ⊢ e _ ∈ <{ [ α := τ' ] τ }>
-where "Δ ; Γ '⊢' t '∈' T" := (typing_judgment Δ Γ t T).
+Require Import List.
+Definition tcontext := list ty.
+Inductive typing_judgment : tcontext -> expr -> ty -> Prop :=
+| T_Unit: forall Δ, Δ ⊢ tt ∈ ()
+| T_Var: forall Δ x, x < length Δ -> Δ ⊢ (expr_var x) ∈ (nth x Δ (ids 0))
+| T_Prod: forall Δ e1 τ1 e2 τ2,
+  Δ ⊢ e1 ∈ τ1 ->
+    Δ ⊢ e2 ∈ τ2 ->
+      Δ ⊢ ⟨e1, e2⟩ ∈ <{ τ1 × τ2 }>
+| T_Fst: forall Δ e τ1 τ2,
+  Δ ⊢ e ∈ <{ τ1 × τ2 }> ->
+    Δ ⊢ fst e ∈ τ1
+| T_Snd: forall Δ e τ1 τ2,
+  Δ ⊢ e ∈ <{ τ1 × τ2 }> ->
+    Δ ⊢ snd e ∈ τ2
+| T_Lam: forall Δ e τ1 τ2,
+  (τ1 :: Δ) ⊢ e ∈ τ2 ->
+    Δ ⊢ (expr_lam e) ∈ <{ τ1 -> τ2 }>
+| T_App: forall Δ f e τ1 τ2,
+  Δ ⊢ f ∈ <{ τ1 -> τ2 }> ->
+    Δ ⊢ e ∈ τ1 ->
+      Δ ⊢ f e ∈ τ2
+| T_TLam: forall Δ e τ,
+  Δ..[ren (+1)] ⊢ e ∈ τ ->
+          Δ ⊢ Λ e ∈ <{ ∀ _ , τ }>
+| T_TApp: forall Δ e τ τ',
+  Δ ⊢ e ∈ <{ ∀ _ , τ }> ->
+  typing_judgment Δ (expr_tapp e) τ.[τ'/]
+where "Δ '⊢' e '∈' τ" := (typing_judgment Δ e τ).
 
 Notation "( x )" := x (in custom sf, x at level 99).
 
@@ -253,9 +166,9 @@ Lemma is_val_inversion : forall e, is_val e -> exists v, e = (of_val v).
 Proof.
   intros.
   induction e;inversion H
-  ;[ exists val_unit | | eexists (val_abs _ _)
-     | eexists (val_tabs _) ]; eauto.
+  ;[ exists val_unit | | eexists (val_lam _ )
+     | eexists (val_tlam _) ]; eauto.
   apply IHe1 in H2; apply IHe2 in H3.
   destruct H2; destruct H3; subst.
-  exists (val_pair x0 x1); eauto.
+  exists (val_pair x x0); eauto.
 Qed.
